Some in-progress proofs trying out pd construction

proofs/core/ADTSpec.v
@@ -7,6 +7,8 @@
 Plan:
 X 1. Define these properties generally
 2. Refactor existing proofs to use these properties instead of fixing to W-types
+  NOTE: I think this will require the isomorphism already to give us the changing-context theorems
+  TODO: let's start with the isomorphism
 3. Prove that W-types satisfy these properties (probably need construction)
   NOTE: might involve following
   a. define construction
@@ -20,7 +22,7 @@ X 1. Define these properties generally
 
 Goal: sound reasoning about Why3 proof terms via shallowly embedded Rocq terms
   *)
-Require Import Hlist Typing Domain. (*TODO: remove*)
+Require Export Hlist Typing Domain. (*TODO: remove*)
 
 Definition fun_interp (pd: sort -> Set) := forall (f:funsym) (srts: list sort)
     (a: arg_list (domain pd) (sym_sigma_args f srts)),
@@ -89,6 +91,436 @@ Record adt_interp_props {gamma: context} (gamma_valid: valid_context gamma)
     ),
     forall t t_in (x: adt_rep pd t srts), P t t_in x;
   }.
+
+Require Import IndTypes.
+
+Check adt_rep.
+
+Search context option mut_adt.
+
+Search sort "ind".
+
+Print sort.
+Print vty.
+
+(*TODO: move*)
+Definition mk_Forall {A: Type} {P: A -> Prop} := 
+  fun (f: forall x, P x) =>
+    fix mk_Forall (l: list A) {struct l} : Forall P l :=
+      match l with
+      | nil => Forall_nil _
+      | x :: xs => Forall_cons _ _ _ (f x) (mk_Forall xs)
+      end.
+
+Definition mk_ForallT {A: Type} {P: A -> Type} := 
+  fun (f: forall x, P x) =>
+    fix mk_ForallT (l: list A) {struct l} : ForallT P l :=
+      match l with
+      | nil => ForallT_nil _
+      | x :: xs => ForallT_cons _ (f x) (mk_ForallT xs)
+      end.
+
+Unset Elimination Schemes.
+Inductive srt :=
+  | srt_int : srt
+  | srt_real : srt
+  | srt_cons: typesym -> list srt -> srt.
+Set Elimination Schemes.
+
+Fixpoint srt_ind (P: srt -> Prop) (P_int: P srt_int) (P_real: P srt_real) 
+  (P_cons: forall (ts: typesym) (srts: list srt) (IH: Forall P srts), P (srt_cons ts srts))
+  (s: srt) : P s :=
+  match s with
+  | srt_int => P_int
+  | srt_real => P_real
+  | srt_cons ts srts => P_cons ts srts (mk_Forall (srt_ind P P_int P_real P_cons) srts)
+  end.
+
+Fixpoint srt_rect (P: srt -> Type) (P_int: P srt_int) (P_real: P srt_real) 
+  (P_cons: forall (ts: typesym) (srts: list srt) (IH: ForallT P srts), P (srt_cons ts srts))
+  (s: srt) : P s :=
+  match s with
+  | srt_int => P_int
+  | srt_real => P_real
+  | srt_cons ts srts => P_cons ts srts (mk_ForallT (srt_rect P P_int P_real P_cons) srts)
+  end.
+
+Lemma var_not_sort v: ~ is_sort (vty_var v).
+Proof.
+  unfold is_sort. simpl. rewrite aset_singleton_not_empty. auto.
+Qed.
+
+Lemma is_sort_cons_Forall ts l: is_sort (vty_cons ts l) -> Forall is_sort l.
+Proof.
+  rewrite Forall_forall. apply is_sort_cons.
+Qed.
+
+(*The isomorphism*)
+
+Fixpoint sort_to_srt_aux (t: vty) (Hs: is_sort t) : srt :=
+  match t return is_sort t -> srt with
+  | vty_int => fun _ => srt_int
+  | vty_real => fun _ => srt_real
+  | vty_var v => fun Hs => False_rect _ (var_not_sort _ Hs)
+  | vty_cons ts tys => fun Hs => srt_cons ts (dep_map sort_to_srt_aux tys (is_sort_cons_Forall _ _ Hs))
+  end Hs.
+
+Definition sort_to_srt (s: sort) : srt := sort_to_srt_aux (proj1_sig s) (proj2_sig s).
+
+Fixpoint srt_to_ty (s: srt) : vty :=
+  match s with
+  | srt_int => vty_int
+  | srt_real => vty_real
+  | srt_cons ts srts => vty_cons ts (map srt_to_ty srts)
+  end.
+
+Lemma srt_to_ty_sort s: is_sort (srt_to_ty s).
+Proof.
+  induction s; simpl; auto.
+  apply is_sort_cons_iff.
+  rewrite <- Forall_forall, Forall_map.
+  exact IH.
+Qed.
+
+Definition srt_to_sort (s: srt) : sort := exist is_sort _ (srt_to_ty_sort s).
+
+Set Bullet Behavior "Strict Subproofs".
+
+Lemma srt_to_sort_to_srt s:
+  sort_to_srt (srt_to_sort s) = s.
+Proof.
+  unfold sort_to_srt, srt_to_sort. simpl.
+  generalize dependent (srt_to_ty_sort s).
+  induction s; simpl; try reflexivity.
+  intros Hsort. f_equal.
+  generalize dependent (is_sort_cons_Forall ts (map srt_to_ty srts) Hsort).
+  induction srts as [| s stl IHs]; simpl; auto.
+  intros f. inversion IH as [| ? ? Hs Hst]; subst. 
+  f_equal.
+  - apply Hs.
+  - apply IHs; auto. inversion f; subst. 
+    rewrite is_sort_cons_iff, <- Forall_forall.
+    assumption.
+Qed.
+
+Lemma sort_to_srt_to_sort s:
+  srt_to_sort (sort_to_srt s) = s.
+Proof.
+  unfold srt_to_sort, sort_to_srt. apply sort_inj. simpl.
+  destruct s as [ty Hsort]. simpl.
+  revert Hsort.
+  induction ty as [| | v | ts tys IHtys]; simpl; auto.
+  - intros Hsort. exfalso. apply (var_not_sort _ Hsort).
+  - intros Hsort. f_equal. rewrite map_dep_map.
+    generalize dependent (is_sort_cons_Forall ts tys Hsort).
+    clear Hsort. induction tys as [| x tl IHtl]; simpl; auto.
+    intros Hall. inversion IHtys as [| ? ? Hx Htl]; subst.
+    inversion Hall as [| ? ? Hsx Hstl]; subst.
+    f_equal; auto.
+Qed.
+
+Lemma srt_to_sort_int: srt_to_sort srt_int = s_int.
+Proof.
+  apply sort_inj. reflexivity.
+Qed.
+
+Lemma srt_to_sort_real: srt_to_sort srt_real = s_real.
+Proof.
+  apply sort_inj. reflexivity.
+Qed.
+
+Lemma srt_to_sort_cons ts srts: srt_to_sort (srt_cons ts srts) = typesym_to_sort ts (map srt_to_sort srts).
+Proof.
+  apply sort_inj. simpl. f_equal.
+  induction srts as [| x t IH]; simpl; auto.
+  f_equal. auto.
+Qed.
+
+(*And now an induction principle on sorts*)
+Lemma sort_ind (P: sort -> Prop) (P_int: P s_int) (P_real: P s_real)
+  (P_cons: forall (ts: typesym) (srts: list sort) (IH: Forall P srts), P (typesym_to_sort ts srts))
+  (s: sort) : P s.
+Proof.
+  set (s' := sort_to_srt s).
+  set (P' := fun (s: srt) => P (srt_to_sort s)).
+  assert (Hp: P' s'). {
+    apply srt_ind.
+    - unfold P'. rewrite srt_to_sort_int. exact P_int.
+    - unfold P'. rewrite srt_to_sort_real. exact P_real.
+    - intros ts srts. unfold P'. rewrite srt_to_sort_cons. intros Hall. 
+      apply P_cons; rewrite Forall_map; auto.
+  }
+  unfold P', s' in Hp. rewrite sort_to_srt_to_sort in Hp.
+  exact Hp.
+Qed.
+
+(*Note: opaque for now*)
+Lemma ForallT_map1 {A B: Type} (f: A -> B) (P: B -> Type) (l: list A):
+  ForallT P (map f l) -> ForallT (fun x => P (f x)) l.
+Proof.
+  induction l as [| h t IH].
+  - constructor.
+  - intros Hall. inversion Hall; subst. constructor; auto.
+Qed. 
+
+Lemma ForallT_map2 {A B: Type} (f: A -> B) (P: B -> Type) (l: list A):
+  ForallT (fun x => P (f x)) l -> ForallT P (map f l).
+Proof.
+  induction l as [| h t IH].
+  - constructor.
+  - intros Hall. inversion Hall; subst. constructor; auto.
+Qed. 
+
+(*Opaque*)
+Lemma sort_rect (P: sort -> Type) (P_int: P s_int) (P_real: P s_real)
+  (P_cons: forall (ts: typesym) (srts: list sort) (IH: ForallT P srts), P (typesym_to_sort ts srts))
+  (s: sort) : P s.
+Proof.
+  set (s' := sort_to_srt s).
+  set (P' := fun (s: srt) => P (srt_to_sort s)).
+  assert (Hp: P' s'). {
+    apply srt_rect.
+    - unfold P'. rewrite srt_to_sort_int. exact P_int.
+    - unfold P'. rewrite srt_to_sort_real. exact P_real.
+    - intros ts srts. unfold P'. rewrite srt_to_sort_cons. intros Hall. 
+      apply P_cons. apply ForallT_map2. exact Hall.
+  }
+  unfold P', s' in Hp. rewrite sort_to_srt_to_sort in Hp.
+  exact Hp.
+Qed.
+
+(*TODO: just use recursive sort*)
+Lemma sort_rect_int P P_int P_real P_cons:
+  sort_rect P P_int P_real P_cons s_int = P_int.
+Proof. Admitted.
+
+Lemma sort_rect_real P P_int P_real P_cons:
+  sort_rect P P_int P_real P_cons s_real = P_real.
+Proof. Admitted.
+
+Lemma sort_rect_typesym_to_sort P P_int P_real P_cons ts srts:
+  sort_rect P P_int P_real P_cons (typesym_to_sort ts srts) = 
+  P_cons ts srts (mk_ForallT (sort_rect P P_int P_real P_cons) srts).
+Admitted.
+
+Definition ts_map_to_pd (f: typesym -> list sort -> Set) : sort -> Set :=
+  sort_rect (fun _ => Set) Z R (fun ts srts IH => f ts srts).
+
+(* Lemma ts_map_to_pd_domain f:
+   *)
+
+Print adt_rep.
+
+Definition adt_rep' (m: mut_adt) (srts: list sort) (d1 d2: sort -> Set) (a: alg_datatype)
+  (a_in: adt_in_mut a m) :=
+  mk_adts (var_map m srts d1) (typesym_map m srts d2) (adts m) (get_idx adt_dec a (adts m) a_in).
+
+Fixpoint mk_ts_map (gamma: context) (pd: sort -> Set) (n: nat) (ts: typesym) (srts: list sort) : Set :=
+  match n with
+  | O => pd (typesym_to_sort ts srts)
+  | S n' =>
+    let pd' := ts_map_to_pd (mk_ts_map gamma pd n')
+(*     sort_rect (fun _ => Set) Z R (fun ts srts IH => mk_ts_map gamma n' pd ts srts) *)
+     (*  let fix f (s: srt) : Set :=
+      match s with
+      | srt_int => Z
+      | srt_real => R
+      | srt_cons ts srts => mk_ts_map gamma n' f ts (map srt_to_sort srts)
+      end in
+      f (sort_to_srt s) *)
+    in
+    match find_ts_in_ctx gamma ts as b return find_ts_in_ctx gamma ts = b -> _ with
+    | Some (m, a) => fun Hfind => adt_rep' m srts pd' pd a (proj1 (proj2 (find_ts_in_ctx_some _ _ _ _ Hfind)))
+    | None => fun _ => pd (typesym_to_sort ts srts)
+    end eq_refl
+    end.
+
+Definition mk_pd_aux (gamma: context) (pd: sort -> Set) (n: nat) (s: sort) : Set :=
+  ts_map_to_pd (mk_ts_map gamma pd n) s.
+
+(*Idea: should be invariant as long as n larger than max depth of sort*)
+Fixpoint srt_depth (s: srt) : nat :=
+  match s with
+  | srt_int => 1
+  | srt_real => 1
+  | srt_cons ts srts => 1 + list_max (map srt_depth srts)
+  end.
+
+Definition srts_depth (s: list srt) : nat := list_max (map srt_depth s).
+
+Definition sort_depth s := srt_depth (sort_to_srt s).
+Definition sorts_depth s := srts_depth (map sort_to_srt s).
+
+Definition mk_ts_full gamma pd ts srts :=
+  mk_ts_map gamma pd (sorts_depth srts) ts srts.
+
+Definition mk_pd (gamma: context) (pd: sort -> Set) (s: sort) : Set :=
+  ts_map_to_pd (mk_ts_full gamma pd) s.
+
+
+(*pd with all typesym_to_sort set correctly to the corresponidng W-type*)
+Definition pd_full (gamma: context) (pd: sort -> Set) := forall (m: mut_adt) (srts: list sort)
+    (a: alg_datatype) (m_in: mut_in_ctx m gamma) (Hin: adt_in_mut a m),
+    pd (typesym_to_sort (adt_name a) srts) =
+    adt_rep m srts pd a Hin.
+
+Definition pd_full_aux (gamma: context) (pd: sort -> Set) (n: nat) := forall (m: mut_adt) (srts: list sort)
+    (a: alg_datatype) (m_in: mut_in_ctx m gamma) (Hin: adt_in_mut a m) ,
+    1 + sorts_depth srts < n ->
+    pd (typesym_to_sort (adt_name a) srts) =
+    adt_rep m srts pd a Hin.
+
+Lemma mk_ts_map_invar gamma pd n1 n2 s:
+  sort_depth s < n1 ->
+  sort_depth s < n2 ->
+  ts_map_to_pd (mk_ts_map gamma pd n1) s = ts_map_to_pd (mk_ts_map gamma pd n2) s.
+Proof.
+  generalize dependent n2. generalize dependent s. induction n1 as [| n1 IHn1].
+  { intros; lia. }
+  intros s [| n2]; [lia | intros Hn1 Hn2].
+  unfold ts_map_to_pd.
+  (*TODO: need recursive sorts*)
+  assert (Hs: s = s_int \/ s = s_real \/ exists ts srts, s = typesym_to_sort ts srts). { admit. }
+  destruct Hs as [Hs | [Hs | [ts [srts Hs]]]].
+  - subst. rewrite !sort_rect_int. reflexivity.
+  - subst. rewrite !sort_rect_real. reflexivity.
+  - subst. rewrite !sort_rect_typesym_to_sort. simpl.
+    simpl. generalize dependent (find_ts_in_ctx_some gamma ts).
+    destruct (find_ts_in_ctx gamma ts) as [[m a]|] eqn : Hfind; auto.
+    intros H. generalize dependent (proj1 (proj2 (H m a eq_refl))). clear H.
+    intros a_in. unfold adt_rep'.
+    f_equal. apply functional_extensionality. intros x.
+    unfold var_map. unfold domain. unfold sigma. simpl.
+    destruct (in_dec string_dec x (m_params m)) as [Hin| Hin].
+    + (*Case 1: if var in list, maps to corresponding sort, which has smaller size than n1 and n2,
+        so use IH*)
+      (*Note: we need a lemma that doesnt require length eq, as long as in both lists, otherwise prove default
+        for now just admit*)
+      destruct (In_nth _ _ EmptyString Hin) as [n [Hn Hx]].
+      subst. rewrite ty_subst_fun_nth with (s:=vty_int); auto.
+      2: { (*here*) admit. }
+      2: { apply m_params_Nodup. }
+      unfold sorts_to_tys. rewrite !(map_nth_inbound) with (d2:=s_int); auto. 2: admit.
+      destruct (sort_to_ty (nth n srts s_int)) eqn : Hs; auto.
+      { (*sort not var*) unfold sort_to_ty in Hs. destruct (nth n srts s_int); simpl in Hs. subst.
+        exfalso. apply (var_not_sort t); auto. }
+      unfold ty_subst_s. unfold v_subst. simpl. apply IHn1.
+      * (*identical proofs*)
+        unfold sort_depth. unfold sort_to_srt. simpl.
+        match goal with |- context [ sort_to_srt_aux ?x ?y] => generalize dependent y end.
+        simpl. rewrite !ty_subst_fun_nth with (s:=vty_int); auto.
+        2: { admit. } 2: { apply m_params_Nodup. }
+        unfold sorts_to_tys. rewrite !map_nth_inbound with (d2:=s_int) by admit.
+        (*TODO: this is doable once we have recursive sorts*)
+        admit.
+      * (*similar*) admit.
+    + rewrite !ty_subst_fun_notin; auto.
+Admitted.
+
+
+
+(*Lemma mk_ts_map_change_n (gamma: context) (pd: sort -> Set) (n1 n2: nat) (ts: typesym) (srts: list sort)
+  (Hn1: sorts_depth srts < n1)
+  (Hn2: sorts_depth srts < n2):
+  mk_ts_map gamma pd n1 ts srts = mk_ts_map gamma pd n2 ts srts.
+Proof.
+  generalize dependent n2. generalize dependent srts. induction n1 as [| n1 IHn1].
+  - intros; lia.
+  - intros srts Hn1 [| n2]; [lia|]; intros Hn2.
+    simpl. generalize dependent (find_ts_in_ctx_some gamma ts).
+    destruct (find_ts_in_ctx gamma ts) as [[m a]|] eqn : Hfind; auto.
+    intros Hdefs. generalize dependent (proj1 (proj2 (Hdefs m a eq_refl))).
+    intros a_in. clear Hdefs.
+    (*Now we need to show we can change adt_rep pd*)
+
+
+
+    (*TODO: separate lemma*)
+    unfold adt_rep.
+    Print mk_adts.
+    Print typesym_map.
+
+Lemma mk_adts_ext (
+    unfold var_map.
+   
+    
+
+ specialize (Hdefs m a eq_refl).
+  
+
+Lemma mk_pd_aux_change_n gamma pd n1 n2:*)
+
+Check adt_rep.
+Lemma adt_rep_eq m srts pd a a_in:
+  adt_rep' m srts pd pd a a_in = adt_rep m srts pd a a_in.
+Proof. reflexivity. Qed.
+
+Search mk_adts.
+(*Now we will try to prove for the generalized version*)
+Lemma mk_pd_aux_full gamma pd n: valid_context gamma -> pd_full_aux gamma (mk_pd_aux gamma pd n) n.
+Proof.
+  intros gamma_valid.
+  unfold pd_full_aux, mk_pd_aux. unfold ts_map_to_pd at 1. intros m srts a m_in a_in Hn.
+  rewrite sort_rect_typesym_to_sort.
+  (*TODO: could I prove that this equals mk_ts ... (pred n) (bc if n large enough, doesn't change)
+    *)
+  assert (Htest: forall pd', adt_rep' m srts (fun s : sort => ts_map_to_pd (mk_ts_map gamma pd n) s) pd' a a_in =
+    adt_rep' m srts (fun s : sort => ts_map_to_pd (mk_ts_map gamma pd (pred n)) s) pd' a a_in).
+  {
+    unfold adt_rep'. intros pd'. f_equal. apply functional_extensionality. intros x.
+    (*TODO: prove var_map result as separate lemma after previous (which we needed for induction, we needed sort
+      explicitly)*)
+    admit.
+  }
+  rewrite <- adt_rep_eq.
+  rewrite Htest. clear Htest.
+  generalize dependent srts. induction n as [| n' IH].
+  - intros; lia.
+  - intros srts Hdepth. (*TODO: generalize pd in [adt_rep]?*) simpl.
+    generalize dependent (find_ts_in_ctx_some gamma (adt_name a)).
+    assert (Hfind: find_ts_in_ctx gamma (adt_name a) = Some (m, a)). {
+      apply find_ts_in_ctx_iff; auto.
+    }
+    rewrite Hfind.
+    intros H.
+    assert (Heq: (proj1 (proj2 (H m a eq_refl))) = a_in) by (apply bool_irrelevance).
+    rewrite Heq.
+
+    (*I think we need a result (not sure if provable): for d2, if agrees on all 
+      typesyms that are NOT in the ADT in question, then same (tying knot lemma)
+      then need to show agrees on all typesyms not in ADT for all n, then connect with n = 0
+      this lemma should be true, hopefully it is provable
+*)
+
+ clear H Heq.
+    reflexivity.
+
+(*So plan is this:
+  1. If n1 and n2 are larger than depth, show that we can change n
+  2. show we can change in adt_rep *)
+
+    unfold adt_rep. 
+    
+
+ specialize (H m a eq_refl).
+
+
+find_ts_in_ctx_iff
+    Search find_ts_in_ctx.
+    destruct (find_ts_in_ctx gamma (adt_name a)) as [ eqn : Hfind.
+
+ eqn : Hfind.
+ unfold mk_ts_map at 1.
+  
+
+
+  unfold sort_rect. simpl. intros m srts a m_in a_in Hn.
+
+    
+
+(*Going to prove 2 things:
+  1. If we assume adts and constrs conditions hold, then we get [adt_interp_props]
+  2. We can construct pd and pf st adts and constrs hold by assigning ADT_rep*)
 
 (* constrs_disj: forall {m1 m2: mut_adt} {a1 a2: alg_datatype} {f1 f2: funsym} 
     (m1_in: mut_in_ctx m1 gamma) (m2_in: mut_in_ctx m2 gamma) 
